PoS/Invariants.v
@@ -71,15 +71,15 @@ Lemma local_chain_grows_fork_step (w w' : World) q n bc bc':
   bc = bc' \/ (([bc <<< bc'] \/ fork bc bc') /\ bc' > bc).
 Proof.
 move=>D H1 S H2; move: (Coh_step S)=>C2.
-case: S=>[[C]Z|p [n' prs bt pool] C _ _ F|
-          proc t s1 C _ F].
+case: S=>[[C]Z|p [n' prs bt pool] [c1 c2 c3] _ _ F|
+          proc t s1 [c1 c2 c3] _ F].
 
 (* 0 steps *)
 - by subst w'; rewrite (has_chain_func D H1 H2); left.
 (* Step is procedding a message *)
 
 (* Receiving a message *)
-- have E: (n' = (dst p)) by case:C=>_/(_ (dst p) _ F)/eqP. subst n'.
+- have E: (n' = (dst p)) by move/eqP: (c2 (dst p) _ F). subst n'.
 
   (* Two sub-cases: (dst p) =? n *)
   case N : (n == dst p);[move/eqP:N=>N; subst n|]; last first.
@@ -90,7 +90,7 @@ case: S=>[[C]Z|p [n' prs bt pool] C _ _ F|
   rewrite [procMsg _ _ _]surjective_pairing=>Z;
   (* Avoiding premature unfolding. *)
   set Pm := nosimpl (procMsg _ _ _) in Z; subst w'.
-  rewrite /holds/= findU eqxx/= (proj1 (C)) in H2.
+  rewrite /holds/= findU eqxx/= c1 in H2.
   move/(H2 Pm.1): (erefl (Some Pm.1))=>{H2} H2.
   move: (H1 _ F)=>{H1 C2 F}/=H1.
   by apply: (@procMsg_bc_prefix_or_fork bc bc'
@@ -109,7 +109,7 @@ case N : (n == proc);[move/eqP:N=>N; subst n|]; last first.
    Don't hesitate to introduce auxiliary lemmas. *)
 rewrite [procInt _ _ _]surjective_pairing=>Z.
 set Pi := nosimpl (procInt _ _ _) in Z; subst w'.
-rewrite /holds/= findU eqxx/= (proj1 (C)) in H2. rewrite /holds F in H1.
+rewrite /holds/= findU eqxx/= c1 in H2. rewrite /holds F in H1.
 have: (Some s1 = Some s1). by []. move=> eq. move: (H1 s1 eq)=>hbc. clear eq.
 have: (Some Pi.1 = Some Pi.1). by []. move=> eq. move: (H2 Pi.1 eq)=>hbc'. clear eq.
 rewrite /has_chain in hbc hbc'. move/eqP in hbc. move/eqP in hbc'.
@@ -335,7 +335,8 @@ Lemma Inv_step w w' q :
   Inv w -> system_step w w' q -> Inv w'.
 Proof.
 move=>Iw S; rewrite/Inv; split; first by apply: (Coh_step S).
-case: S=>[|p st1 Cw _ iF Fw|proc t st1 Cw _ Fw]; first by elim=>_ <-; move: Iw=>[].
+case: S=>[|p st1 [c1 c2 c3] _ iF Fw|proc t st1 [c1 c2 c3] _ Fw];
+  first by elim=>_ <-; move: Iw=>[].
 case: Iw=>_ [GStabW|GSyncW].
 - by case GStabW=>noPackets; contradict iF; rewrite noPackets.
 - case GSyncW=>can_bc [can_n] [] HHold HGt HInFlight HDiffAv.
@@ -350,17 +351,18 @@ case: Iw=>_ [GStabW|GSyncW].
     rewrite/holds/localState/has_chain=>st';
     case X: (can_n == dst p); move/eqP in X;
     (* All cases except BlockMsg *)
-    do? [subst can_n; rewrite findU (proj1 Cw)=>/=; case: ifP;
+    do? [subst can_n; rewrite findU c1=>/=; case: ifP;
       by [move/eqP |
         NBlockMsg_dest q st1 p b Msg H; rewrite Msg P=><-; apply (HHold st1 Fw)
     ]];
-    do? [rewrite findU (proj1 Cw)=>/=; case: ifP=>/=;
+    do? [rewrite findU c1=>/=; case: ifP=>/=;
       by [move/eqP | move=>_ Fc; move: (HHold st' Fc)]
     ].
     (* BlockMsg *)
-    rewrite findU (proj1 Cw)=>/=; case: ifP=>/=; last by move/eqP.
+    rewrite findU c1=>/=; case: ifP=>/=; last by move/eqP.
     BlockMsg_dest w q can_n can_bc st1 p iF Fw P Msg b X HHold HInFlight.
-    * by move=>H; move: (btExtend_seq_same X H); move/eqP; rewrite eq_sym.
+    move: (c3 (dst p) _ Fw)=>V.
+    * by move=>H; move: (btExtend_seq_same V X H); move/eqP; rewrite eq_sym.
     * by move=>Con; contradict Con; apply btExtend_fold_not_worse.
 
  (* ... it's still the largest *)
@@ -368,14 +370,15 @@ case: Iw=>_ [GStabW|GSyncW].
     (* All cases except BlockMsg *)
     rewrite/holds/localState/has_chain=>n' bc' st';
     case X: (can_n == dst p); move/eqP in X;
-    rewrite findU (proj1 Cw)=>/=; case: ifP=>/=; move/eqP;
+    rewrite findU c1=>/=; case: ifP=>/=; move/eqP;
     do? by [
       move=>_ Fc; move: (HGt n' bc' st' Fc) |
       NBlockMsg_dest q st1 p b Msg H; rewrite /has_chain Msg P=><-;
       rewrite -Eq in Fw=>Hc; move: (HGt n' bc' st1 Fw Hc)].
     (* BlockMsg *)
     BlockMsg_dest w q can_n can_bc st1 p iF Fw P Msg b X HHold HInFlight.
-    * by move=>H; move: (btExtend_seq_same X H)=><-/eqP->; left.
+    move: (c3 (dst p) _ Fw)=>V.
+    * by move=>H; move: (btExtend_seq_same V X H)=><-/eqP->; left.
     * by move=>Con; contradict Con; apply btExtend_fold_not_worse.
 
     (* TODO: Make this shorter! *)
@@ -388,7 +391,8 @@ case: Iw=>_ [GStabW|GSyncW].
     specialize (HGt (dst p) (btChain (blockTree st1)) _ Fw).
     rewrite/has_chain eqxx in HGt.
     (have: (is_true true) by done)=>Obvs; specialize (HGt Obvs); clear Obvs.
-    by move: (btExtend_seq_sameOrBetter_fref X HGt HInFlight).
+    move: (c3 (dst p) _ Fw)=>V.
+    by move: (btExtend_seq_sameOrBetter_fref V X HGt HInFlight).
 
 (* the canonical chain can only change throught a MintT transition *)
 (* TODO: refactor it into a lemma *)
